Disaster

transaction_kohler.v
@@ -17,7 +17,7 @@ Definition value := nat.
 Definition lock := bool.
 Definition variable := nat.
 Definition store := NatMap.t value.
-Definition heap :=  address -> option (value * lock * version).
+Definition heap := address -> option (value * lock * version).
 Definition tid := nat.
 
 
@@ -69,14 +69,20 @@ Definition action_phase (a:action) :=
   | unlock_write_item => 6
   end.
 
-Fixpoint trace_tid_phase tid t: nat :=
+Fixpoint tid_phase tid t: nat :=
   match t with
   | (tid', a) :: t' =>
     if Nat.eq_dec tid tid'
     then action_phase a
-    else trace_tid_phase tid t'
+    else tid_phase tid t'
   | [] => 0
   end.
+
+Lemma tid_phase_head tid a t:
+  tid_phase tid ((tid, a) :: t) = action_phase a.
+Proof.
+  cbn; destruct (Nat.eq_dec tid tid); congruence.
+Qed.
 
 (* Return the version number of the last committed write *)
 Fixpoint trace_write_version (t:trace): version :=
@@ -114,28 +120,28 @@ Inductive sto_trace : trace -> Prop :=
 
 | start_txn_step: forall t tid,
     tid > 0
-    -> trace_tid_phase tid t = 0
+    -> tid_phase tid t = 0
     -> sto_trace t
     -> sto_trace ((tid, start_txn)::t)
 
 | read_item_step: forall t tid,
-    trace_tid_phase tid t = 1
+    tid_phase tid t = 1
     -> locked_by t 0 = 0
     -> sto_trace t
     -> sto_trace ((tid, read_item (trace_write_version t)) :: t)
 
 | write_item_step: forall t tid val,
-    trace_tid_phase tid t = 1
+    tid_phase tid t = 1
     -> sto_trace t
     -> sto_trace ((tid, write_item val) :: t)
 
 | try_commit_txn_step: forall t tid,
-    trace_tid_phase tid t = 1
+    tid_phase tid t = 1
     -> sto_trace t
     -> sto_trace ((tid, try_commit_txn)::t)
 
 | lock_write_item_step: forall t tid v,
-    trace_tid_phase tid t = 2
+    tid_phase tid t = 2
     -> In (tid, write_item v) t
     -> locked_by t 0 = 0
     -> sto_trace t
@@ -143,47 +149,47 @@ Inductive sto_trace : trace -> Prop :=
 
 (*sequential point*)
 | seq_point_step: forall t tid,
-    trace_tid_phase tid t = 2
+    tid_phase tid t = 2
     -> (forall v, In (tid, write_item v) t
                   -> In (tid, lock_write_item) t)
     -> sto_trace t
     -> sto_trace ((tid, seq_point) :: t)
 
 | validate_read_item_step: forall t tid vers,
-    trace_tid_phase tid t = 3
+    tid_phase tid t = 3
     -> locked_by t tid = tid (* unlocked or locked by me *)
     -> trace_write_version t = vers
     -> sto_trace t
     -> sto_trace ((tid, validate_read_item vers) :: t)
 
 | abort_txn_step: forall t tid,
-    trace_tid_phase tid t > 0
-    -> trace_tid_phase tid t < 4
+    tid_phase tid t > 0
+    -> tid_phase tid t < 4
     -> sto_trace t
     -> sto_trace ((tid, abort_txn) :: t)
 
 | unlock_item_step: forall t tid,
-    trace_tid_phase tid t = 6
+    tid_phase tid t = 6
     -> locked_by t 0 = tid
     -> sto_trace t
     -> sto_trace ((tid, unlock_write_item) :: t)
 
 | commit_txn_step: forall t tid,
-    trace_tid_phase tid t = 3
+    tid_phase tid t = 3
     -> (forall vers, In (tid, read_item vers) t
                      -> In (tid, validate_read_item vers) t)
     -> sto_trace t
     -> sto_trace ((tid, commit_txn) :: t)
 
 | complete_write_item_step: forall t tid val,
-    trace_tid_phase tid t = 4
+    tid_phase tid t = 4
     -> locked_by t 0 = tid
     -> trace_tid_last_write tid t = Some val
     -> sto_trace t
     -> sto_trace ((tid, complete_write_item (S (trace_write_version t))) :: t)
 
 | commit_done_step: forall t tid,
-    trace_tid_phase tid t = 4
+    tid_phase tid t = 4
     -> locked_by t 0 <> tid
     -> ~ In (tid, commit_done_txn) t
     -> sto_trace t
@@ -219,27 +225,16 @@ The first element (tid) of the sequence is the first transaction that completes 
 Note that STO-trace is constructed in a reverse order: the first (tid * action) pair is the last operation in the trace
 *)
 
-Function seq_list (sto_trace: trace): list nat:=
-  match sto_trace with
-  | [] => []
-  | (tid, seq_point) :: tail => seq_list tail ++ [tid]
-  | _ :: tail => seq_list tail
-  end.
-
-Eval compute in seq_list example_txn.
-
-Eval compute in seq_list example_txn2.
-
 Lemma phase_increase_head tid a t:
   sto_trace ((tid, a) :: t) ->
-  action_phase a >= trace_tid_phase tid t.
+  action_phase a >= tid_phase tid t.
 Proof.
   intros; inversion H; cbn; omega.
 Qed.
 
 Lemma phase_increase_app tid t1 t2:
   sto_trace (t1 ++ t2) ->
-  trace_tid_phase tid (t1 ++ t2) >= trace_tid_phase tid t2.
+  tid_phase tid (t1 ++ t2) >= tid_phase tid t2.
 Proof.
   induction t1; intros.
   - simpl; omega.
@@ -254,12 +249,12 @@ Qed.
 Lemma phase_increase_in tid a t:
   sto_trace t ->
   In (tid, a) t ->
-  trace_tid_phase tid t >= action_phase a.
+  tid_phase tid t >= action_phase a.
 Proof.
   intros H I; apply in_split in I.
   destruct I as [l1 [l2 L]].
-  assert (trace_tid_phase tid ((tid, a) :: l2) = action_phase a). {
-    cbn; destruct (Nat.eq_dec tid tid); omega.
+  assert (tid_phase tid ((tid, a) :: l2) = action_phase a). {
+    apply tid_phase_head.
   }
   rewrite L in *; rewrite <- H0; now apply phase_increase_app.
 Qed.
@@ -267,7 +262,7 @@ Qed.
 Lemma phase_increase_in_app tid a (t1 t2:trace):
   sto_trace (t1 ++ t2) ->
   In (tid, a) (t1 ++ t2) ->
-  action_phase a > trace_tid_phase tid t2 ->
+  action_phase a > tid_phase tid t2 ->
   In (tid, a) t1.
 Proof.
   intros T I A.
@@ -288,7 +283,7 @@ Proof.
 Qed.
 
 Lemma trace_phase_in tid t:
-  trace_tid_phase tid t > 0 ->
+  tid_phase tid t > 0 ->
   exists a, In (tid, a) t.
 Proof.
   induction t; intros; cbn in *.
@@ -309,7 +304,7 @@ Proof.
   - intros tid' a' H I.
     destruct I; [ | now apply (IHt _ _ (sto_trace_cons _ _ H)) in H0 ].
     subst; inversion H; auto.
-    all: assert (trace_tid_phase tid' t > 0) as GZ by omega.
+    all: assert (tid_phase tid' t > 0) as GZ by omega.
     all: apply trace_phase_in in GZ.
     all: destruct GZ as [a GZ].
     all: now apply (IHt tid' a).
@@ -317,7 +312,7 @@ Qed.
 
 Lemma trace_phase_nonzero tid t:
   sto_trace t ->
-  trace_tid_phase tid t > 0 ->
+  tid_phase tid t > 0 ->
   tid > 0.
 Proof.
   intros T; induction T; intros P; simpl in P.
@@ -346,7 +341,7 @@ Lemma locked_phase tid t:
   sto_trace t ->
   locked_by t 0 = tid ->
   tid > 0 ->
-  trace_tid_phase tid t >= 2.
+  tid_phase tid t >= 2.
 Proof.
   intros T; revert tid; induction T; intros tid L G.
   1: cbn in L; omega.
@@ -359,8 +354,8 @@ Qed.
 
 Lemma commit_phase_cons tid p t:
   sto_trace (p :: t) ->
-  trace_tid_phase tid t = 4 ->
-  trace_tid_phase tid (p :: t) = 4.
+  tid_phase tid t = 4 ->
+  tid_phase tid (p :: t) = 4.
 Proof.
   destruct p as [tid' a]; intros T Fo; inversion T; cbn in *.
   all: destruct (Nat.eq_dec tid tid'); auto.
@@ -369,8 +364,8 @@ Qed.
 
 Lemma commit_phase_app tid t1 t2:
   sto_trace (t1 ++ t2) ->
-  trace_tid_phase tid t2 = 4 ->
-  trace_tid_phase tid (t1 ++ t2) = 4.
+  tid_phase tid t2 = 4 ->
+  tid_phase tid (t1 ++ t2) = 4.
 Proof.
   induction t1; intros.
   now simpl.
@@ -382,8 +377,8 @@ Qed.
 
 Lemma abort_phase_cons tid p t:
   sto_trace (p :: t) ->
-  trace_tid_phase tid t = 6 ->
-  trace_tid_phase tid (p :: t) = 6.
+  tid_phase tid t = 6 ->
+  tid_phase tid (p :: t) = 6.
 Proof.
   destruct p as [tid' a]; intros T Fo; inversion T; cbn in *.
   all: destruct (Nat.eq_dec tid tid'); auto.
@@ -392,8 +387,8 @@ Qed.
 
 Lemma abort_phase_app tid t1 t2:
   sto_trace (t1 ++ t2) ->
-  trace_tid_phase tid t2 = 6 ->
-  trace_tid_phase tid (t1 ++ t2) = 6.
+  tid_phase tid t2 = 6 ->
+  tid_phase tid (t1 ++ t2) = 6.
 Proof.
   induction t1; intros.
   now simpl.
@@ -406,7 +401,7 @@ Qed.
 
 Lemma phase_2_preserves_lock tid t1 t2:
   sto_trace (t1 ++ t2) ->
-  trace_tid_phase tid (t1 ++ t2) = 2 ->
+  tid_phase tid (t1 ++ t2) = 2 ->
   locked_by t2 0 = tid ->
   locked_by (t1 ++ t2) 0 = tid.
 Proof.
@@ -417,7 +412,7 @@ Proof.
   cbn in P; destruct (Nat.eq_dec tid tid').
   - destruct a; simpl in *; try omega.
     + rewrite e in *; clear e tid.
-      assert (trace_tid_phase tid' t2 >= 2). {
+      assert (tid_phase tid' t2 >= 2). {
         apply locked_phase.
         now apply sto_trace_app with (t1:=(tid',try_commit_txn)::t1).
         auto.
@@ -474,12 +469,12 @@ Proof.
   assert (locked_by tx 0 = tid). {
     rewrite Heqtx; now cbn.
   }
-  assert (trace_tid_phase tid tx = 2). {
-    assert (trace_tid_phase tid tx >= 2). {
+  assert (tid_phase tid tx = 2). {
+    assert (tid_phase tid tx >= 2). {
       apply locked_phase; auto.
       now apply sto_trace_app with (t1:=t1a).
     }
-    assert (2 >= trace_tid_phase tid tx). {
+    assert (2 >= tid_phase tid tx). {
       rewrite <- H1.
       now apply phase_increase_app.
     }
@@ -495,7 +490,7 @@ Lemma seq_point_after t1 t2 tid action:
      \/ action = commit_done_txn.
 Proof.
   intros T.
-  assert (trace_tid_phase tid (t1 ++ (tid, commit_txn) :: t2) = 4) as TG4. {
+  assert (tid_phase tid (t1 ++ (tid, commit_txn) :: t2) = 4) as TG4. {
     apply sto_trace_cons in T.
     apply commit_phase_app; auto.
     simpl; destruct (Nat.eq_dec tid tid); congruence.
@@ -551,7 +546,7 @@ Proof.
   destruct a; destruct a.
   all: try solve [ apply IHt1; now apply sto_trace_cons in T ].
   2, 3: omega.
-  assert (trace_tid_phase tid (t1 ++ (tid, commit_done_txn) :: t2) = 4) as P4. {
+  assert (tid_phase tid (t1 ++ (tid, commit_done_txn) :: t2) = 4) as P4. {
     apply commit_phase_app; auto.
     now apply sto_trace_cons in T.
     cbn; destruct (Nat.eq_dec tid tid); congruence.
@@ -565,7 +560,7 @@ Lemma no_steps_after_commit_done tid tid' a t1 t2:
   tid <> tid'.
 Proof.
   intros T.
-  assert (trace_tid_phase tid (t1 ++ (tid, commit_done_txn) :: t2) = 4) as P4. {
+  assert (tid_phase tid (t1 ++ (tid, commit_done_txn) :: t2) = 4) as P4. {
     apply commit_phase_app.
     now apply sto_trace_cons in T.
     cbn; destruct (Nat.eq_dec tid tid); congruence.
@@ -584,3 +579,816 @@ Proof.
     }
     contradiction.
 Qed.
+
+Fixpoint seq_list' (t:trace) (c:list nat) : list nat :=
+  match t with
+  | (tid, commit_txn) :: t' => seq_list' t' (tid :: c)
+  | (tid, seq_point) :: t' =>
+    match count_occ Nat.eq_dec c tid with
+    | 0 => seq_list' t' c
+    | S _ => tid :: seq_list' t' c
+    end
+  | _ :: t' => seq_list' t' c
+  | [] => []
+  end.
+
+Definition seq_list t := seq_list' t [].
+
+Eval compute in seq_list example_txn.
+
+Eval compute in seq_list example_txn2.
+
+Fixpoint serialize_by (t:trace) (c:list nat) : trace :=
+  match c with
+  | tid :: c' =>
+    filter (fun x => if Nat.eq_dec tid (fst x) then true else false) t
+           ++ serialize_by t c'
+  | [] => []
+  end.
+
+Definition serialize (t:trace) : trace :=
+  serialize_by t (seq_list t).
+
+Lemma commit_in_phase4 tid t:
+  sto_trace t ->
+  tid_phase tid t = 4 ->
+  In (tid, commit_txn) t.
+Proof.
+  intros T; induction T; intros P; cbn in *.
+  all: try destruct (Nat.eq_dec tid tid0); try omega.
+  all: try solve [right; now apply IHT].
+  all: subst.
+  1: now left.
+  all: right; now apply IHT.
+Qed.  
+
+Lemma seq_point_in_phase3 tid t:
+  sto_trace t ->
+  tid_phase tid t = 3 ->
+  In (tid, seq_point) t.
+Proof.
+  intros T; induction T; intros P; cbn in *.
+  all: try destruct (Nat.eq_dec tid tid0); try omega.
+  all: try solve [right; now apply IHT].
+  all: subst.
+  1: now left.
+  right; now apply IHT.
+Qed.  
+
+Lemma seq_point_in_commit_head tid t:
+  sto_trace ((tid, commit_txn) :: t) ->
+  In (tid, seq_point) t.
+Proof.
+  intros T; inversion T.
+  apply (seq_point_in_phase3 tid t H3 H1).
+Qed.
+
+Lemma seq_point_in_commit_in tid t1 t2:
+  sto_trace (t1 ++ (tid, commit_txn) :: t2) ->
+  In (tid, seq_point) t2.
+Proof.
+  induction t1; intros; simpl in *.
+  now apply seq_point_in_commit_head.
+  inversion H; now apply IHt1.
+Qed.
+
+Fixpoint remove_tid tid (t:trace) :=
+  match t with
+  | (tid', a) :: t' => if Nat.eq_dec tid tid'
+                       then remove_tid tid t'
+                       else (tid', a) :: remove_tid tid t'
+  | [] => []
+  end.
+
+Lemma in_remove_tid tid tid' a t:
+  tid <> tid' ->
+  In (tid', a) t ->
+  In (tid', a) (remove_tid tid t).
+Proof.
+  induction t; intros NE I; cbn in *; auto.
+  destruct a0; destruct (Nat.eq_dec tid n); destruct or I.
+  inversion I; congruence.
+  auto.
+  now left.
+  right; auto.
+Qed.
+
+Lemma remove_tid_in tid x t:
+  In x (remove_tid tid t) ->
+  In x t.
+Proof.
+  induction t; intros I; cbn in *; auto.
+  destruct a; destruct (Nat.eq_dec tid t0).
+  right; auto.
+  destruct I; [ left | right ]; auto.
+Qed.
+
+Lemma remove_tid_phase tid tid' t:    
+  tid <> tid' ->
+  tid_phase tid' (remove_tid tid t) = tid_phase tid' t.
+Proof.
+  induction t; intros NE; cbn in *; auto.
+  destruct a.
+  destruct (Nat.eq_dec tid t0); destruct (Nat.eq_dec tid' t0);
+    subst; cbn; auto.
+  contradiction.
+  destruct (Nat.eq_dec t0 t0); [ subst; auto | contradiction ].
+  cbn; destruct (Nat.eq_dec tid' t0); [ subst; contradiction | auto ].
+Qed.
+
+Lemma remove_tid_write_version tid t:
+  sto_trace t ->
+  tid_phase tid t <> 4 ->
+  trace_write_version (remove_tid tid t) = trace_write_version t.
+Proof.
+  intros T; induction T; intros P; cbn in *; auto.
+  all: destruct (Nat.eq_dec tid tid0); [ rewrite e in * | ].
+  all: try solve [ apply IHT; omega ].
+  contradiction.
+  now cbn.
+Qed.
+
+Lemma remove_tid_zero t:
+  sto_trace t ->
+  remove_tid 0 t = t.
+Proof.
+  induction t; cbn in *; auto; intros.
+  destruct a.
+  assert (t0 > 0). {
+    apply trace_in_nonzero with (a:=a) (t:=(t0, a)::t); auto.
+    now left.
+  }
+  destruct t0; [ omega | ].
+  assert (sto_trace t) by (inversion H; auto).
+  now rewrite (IHt H1).
+Qed.
+
+Lemma locked_by_unlocked_in tid t:
+  (forall x, In x t -> fst x > 0) ->
+  locked_by t 0 = 0 ->
+  locked_by t tid = tid.
+Proof.
+  induction t; intros A L; cbn in *; auto.
+  destruct a; destruct a.
+  all: try solve [ apply IHt; auto ].
+  assert (n > 0). {
+    replace n with (fst (n, lock_write_item)).
+    apply A; now left.
+    now simpl.
+  }
+  omega.
+  all: reflexivity.
+Qed.
+
+Lemma locked_by_unlocked tid t:
+  sto_trace t ->
+  locked_by t 0 = 0 ->
+  locked_by t tid = tid.
+Proof.
+  intros T L; apply locked_by_unlocked_in; auto.
+  intros x I; destruct x; simpl.
+  now apply (trace_in_nonzero _ a t).
+Qed.
+
+Lemma locked_by_self tid t:
+  sto_trace t ->
+  locked_by t 0 = tid ->
+  locked_by t tid = tid.
+Proof.
+  intros T; induction T; cbn in *; intros L; auto.
+Qed.
+
+Lemma locked_by_other tid tid' t:
+  sto_trace t ->
+  tid' > 0 ->
+  locked_by t 0 = tid' ->
+  locked_by t tid = tid'.
+Proof.
+  intros T; induction T; cbn in *; intros N L; auto.
+  all: omega.
+Qed.
+
+Lemma remove_tid_locked_by_neq tid tid' t:
+  sto_trace t ->
+  locked_by t tid <> tid ->
+  locked_by (remove_tid tid t) tid' = locked_by t tid'.
+Proof.
+  intros T; induction T; intros L; cbn in *; auto.
+  all: destruct (Nat.eq_dec tid tid0); auto.
+  all: congruence.
+Qed.
+
+Lemma remove_tid_locked_by_eq tid tid' t:
+  sto_trace t ->
+  locked_by t tid = tid ->
+  locked_by (remove_tid tid t) tid' = tid'.
+Proof.
+  intros T; induction T; intros L; cbn in *; auto.
+  all: destruct (Nat.eq_dec tid tid0); auto.
+  apply IHT; apply locked_by_unlocked; auto.
+  congruence.
+  all: apply IHT; apply locked_by_self; auto; now rewrite e.
+Qed.
+
+Lemma remove_tid_last_write tid tid' t:
+  tid <> tid' ->
+  trace_tid_last_write tid' (remove_tid tid t) = trace_tid_last_write tid' t.
+Proof.
+  induction t; intros N; cbn in *; auto.
+  destruct a; destruct a;
+    destruct (Nat.eq_dec tid' t0); destruct (Nat.eq_dec tid t0);
+      cbn; auto.
+  all: try congruence.
+  all: destruct (Nat.eq_dec tid' t0); try congruence; auto.
+Qed.
+
+Lemma trace_noncommitted_irrelevant tid t:
+  sto_trace t ->
+  tid_phase tid t <> 4 ->
+  sto_trace (remove_tid tid t).
+Proof.
+  intros T; induction T; intros P; cbn in *; auto.
+  all: destruct (Nat.eq_dec tid tid0);
+    [ subst; try solve [apply IHT; omega] | ].
+  all: try solve
+           [ constructor; auto; rewrite (remove_tid_phase _ _ _ n); auto ].
+
+  {
+    rewrite <- (remove_tid_write_version _ _ T P); constructor.
+    now rewrite remove_tid_phase.
+    rewrite remove_tid_locked_by_eq; auto; now apply locked_by_unlocked.
+    auto.
+  }    
+
+  {
+    apply lock_write_item_step with (v:=v).
+    now rewrite remove_tid_phase.
+    apply in_remove_tid; auto.
+    rewrite remove_tid_locked_by_eq; auto; now apply locked_by_unlocked.
+    auto.
+  }
+
+  {
+    constructor.
+    rewrite (remove_tid_phase _ _ _ n); auto.
+    intros v I.
+    apply in_remove_tid; auto.
+    apply (H0 v).
+    apply (remove_tid_in _ _ _ I).
+    auto.
+  }
+
+  {
+    constructor.
+    rewrite (remove_tid_phase _ _ _ n); auto.
+    destruct (Nat.eq_dec (locked_by t tid) tid);
+      [ rewrite remove_tid_locked_by_eq | rewrite remove_tid_locked_by_neq ];
+      auto.
+    rewrite remove_tid_write_version; auto.
+    auto.
+  }
+
+  {
+    constructor.
+    rewrite (remove_tid_phase _ _ _ n); auto.
+    assert (locked_by t tid <> tid). {
+      rewrite locked_by_other with (tid':=tid0); auto.
+      apply trace_phase_nonzero with (t:=t); auto; omega.
+    }
+    rewrite remove_tid_locked_by_neq; auto.
+    auto.
+  }
+
+  {
+    constructor.
+    rewrite (remove_tid_phase _ _ _ n); auto.
+    intros vers I.
+    apply in_remove_tid; auto.
+    apply H0.
+    apply (remove_tid_in tid); auto.
+    auto.
+  }
+
+  {
+    rewrite <- (remove_tid_write_version _ _ T P).
+    apply complete_write_item_step with (val:=val).
+    now rewrite remove_tid_phase.
+    assert (locked_by t tid <> tid). {
+      rewrite locked_by_other with (tid':=tid0); auto.
+      apply trace_phase_nonzero with (t:=t); auto; omega.
+    }
+    rewrite remove_tid_locked_by_neq; auto.
+    rewrite remove_tid_last_write; auto.
+    auto.
+  }
+
+  {
+    constructor.
+    now rewrite remove_tid_phase.
+    destruct (Nat.eq_dec (locked_by t tid) tid);
+      [ rewrite remove_tid_locked_by_eq | rewrite remove_tid_locked_by_neq ];
+      auto.
+    assert (tid0 > 0). {
+      apply trace_phase_nonzero with (t:=t); auto; omega.
+    }
+    omega.
+    intros I; apply H1; now apply remove_tid_in with (tid0:=tid).
+    auto.
+  }
+Qed.
+
+Lemma tid_phase_swap tid t1 t2 tid1 tid2 a1 a2:
+  tid1 <> tid2 ->
+  tid_phase tid (t1 ++ (tid1, a1) :: (tid2, a2) :: t2) =
+  tid_phase tid (t1 ++ (tid2, a2) :: (tid1, a1) :: t2).
+Proof.
+  induction t1; intros NE; cbn in *; auto.
+  destruct (Nat.eq_dec tid tid1); destruct (Nat.eq_dec tid tid2);
+    congruence.
+  destruct a; destruct (Nat.eq_dec tid n); auto.
+Qed.
+
+Lemma write_version_swap t1 t2 tid1 tid2 a1 a2:
+  action_phase a1 < 4 ->
+  trace_write_version (t1 ++ (tid2, a2) :: (tid1, a1) :: t2) =
+  trace_write_version (t1 ++ (tid1, a1) :: (tid2, a2) :: t2).
+Proof.
+  induction t1; intros AP; cbn in *.
+
+  destruct a1; try solve [ cbn in AP; omega ].
+  1-8: destruct a2; auto.
+
+  destruct a; repeat rewrite (IHt1 AP); auto.
+Qed.
+
+Lemma locked_by_swap_head t1 t2 tid1 tid2 a1 a2 tid:
+  locked_by ((tid2, a2) :: (tid1, a1) :: t2) tid =
+  locked_by ((tid1, a1) :: (tid2, a2) :: t2) tid ->
+  locked_by (t1 ++ (tid2, a2) :: (tid1, a1) :: t2) tid =
+  locked_by (t1 ++ (tid1, a1) :: (tid2, a2) :: t2) tid.
+Proof.
+  induction t1; cbn; auto.
+  intros; destruct a; destruct a.
+  all: try solve [now apply IHt1].
+  all: congruence.
+Qed.
+
+Lemma in_middle_swap_iff {A:Type} (t1 t2:list A) p1 p2 p:
+  In p (t1 ++ p1 :: p2 :: t2) <-> In p (t1 ++ p2 :: p1 :: t2).
+Proof.
+  split; intros.
+  1: apply Permutation_in with (l:=t1 ++ p1 :: p2 :: t2); auto.
+  2: apply Permutation_in with (l:=t1 ++ p2 :: p1 :: t2); auto.
+  all: apply Permutation_app_head.
+  all: now apply perm_swap.
+Qed.
+
+Lemma trace_swap_forward_1 t1 t2 tid1 tid2 a1 a2:
+  sto_trace ((tid1, commit_txn) :: t1 ++ (tid2, a2) :: (tid1, a1) :: t2) ->
+  action_phase a1 < 3 ->
+  tid1 <> tid2 ->
+  sto_trace ((tid1, commit_txn) :: t1 ++ (tid1, a1) :: (tid2, a2) :: t2).
+Proof.
+  revert t2; induction t1; intros t2 T AP N.
+
+  {
+    inversion T.
+    cbn in *.
+    destruct (Nat.eq_dec tid1 tid2); [ congruence | ].
+    destruct (Nat.eq_dec tid1 tid1); [ omega | congruence ].
+  }
+
+  inversion T.
+  constructor.
+  rewrite tid_phase_swap; auto.
+  intros vers I; rewrite in_middle_swap_iff.
+  apply H2; rewrite app_comm_cons; now rewrite in_middle_swap_iff.
+  rewrite <- app_comm_cons.
+  clear tid0 H H0.
+  inversion H3.
+
+  constructor; auto.
+  rewrite tid_phase_swap; auto.
+  apply IHt1.
+  {
+    cbn in *.
+    omega.
+  }
+    rename H3 into T1; inversion T1.
+  
+  inversion H3.
+  inversion H9.
+  simpl.
+  clear T H tid0.
+  rewrite <- H0 in H3.
+  rename H3 into T.
+  revert tid1 tid2 N H1 H2 H0.
+
+
+Lemma trace_swap_forward t1 t2 tid1 tid2 a1 a2:
+  sto_trace (t1 ++ (tid2, a2) :: (tid1, a1) :: t2) ->
+  tid_phase tid1 (t1 ++ (tid2, a2) :: (tid1, a1) :: t2) = 4 ->
+  action_phase a1 < 3 ->
+  tid1 <> tid2 ->
+  sto_trace (t1 ++ (tid1, a1) :: (tid2, a2) :: t2).
+Proof.
+  unfold Top.tid in *.
+  intros T P AP NE; remember (t1 ++ (tid2, a2) :: (tid1, a1) :: t2) as t.
+  revert t1 t2 tid1 tid2 a1 a2 Heqt P AP NE.
+  induction T; intros t1 t2 tid1 tid2 a1 a2 ET P AP NE.
+  destruct t1; cbn in *; discriminate.
+
+  {
+    destruct t1; cbn in *; inversion ET; subst.
+    destruct (Nat.eq_dec tid1 tid2); [ congruence | ].
+    rewrite tid_phase_head in P; omega.
+    destruct (Nat.eq_dec tid1 tid0); [ omega | ].
+
+    constructor; auto.
+    rewrite tid_phase_swap; auto.
+  }
+
+  {
+    destruct t1; cbn in *; inversion ET; subst.
+    destruct (Nat.eq_dec tid1 tid2); [ congruence | ].
+    rewrite tid_phase_head in P; omega.
+    destruct (Nat.eq_dec tid1 tid0); [ omega | ].
+
+    rewrite write_version_swap; auto.
+    constructor; auto.
+    rewrite tid_phase_swap; auto.
+    rewrite locked_by_swap_head; auto.
+
+    assert (sto_trace ((tid2, a2) :: (tid1, a1) :: t2)) as TH. {
+      now apply sto_trace_app with (t1:=t1).
+    }
+    assert (tid1 > 0) as T1N. {
+      apply (trace_in_nonzero _ a1 _ TH).
+      right; now left.
+    }
+    destruct a1; destruct a2; try reflexivity.
+    all: try solve [simpl in AP; omega].
+    all: inversion TH.
+    simpl in H5; omega.
+    simpl in H4; omega.
+    simpl in H5; omega.
+  }
+
+  {
+    destruct t1; cbn in *; inversion ET; subst.
+    destruct (Nat.eq_dec tid1 tid2); [ congruence | ].
+    rewrite tid_phase_head in P; omega.
+    destruct (Nat.eq_dec tid1 tid0); [ omega | ].
+
+    constructor; auto.
+    rewrite tid_phase_swap; auto.
+  }
+
+  {
+    destruct t1; cbn in *; inversion ET; subst.
+    destruct (Nat.eq_dec tid1 tid2); [ congruence | ].
+    rewrite tid_phase_head in P; omega.
+    destruct (Nat.eq_dec tid1 tid0); [ omega | ].
+
+    constructor; auto.
+    rewrite tid_phase_swap; auto.
+  }
+
+  {
+    destruct t1; cbn in *; inversion ET; subst.
+    destruct (Nat.eq_dec tid1 tid2); [ congruence | ].
+    rewrite tid_phase_head in P; omega.
+    destruct (Nat.eq_dec tid1 tid0); [ omega | ].
+
+    apply lock_write_item_step with (v:=v); auto.
+    rewrite tid_phase_swap; auto.
+    apply Permutation_in with (l:=t1 ++ (tid2, a2) :: (tid1, a1) :: t2); auto.
+    apply Permutation_app_head; constructor.
+    rewrite locked_by_swap_head; auto.
+
+    assert (sto_trace ((tid2, a2) :: (tid1, a1) :: t2)) as TH. {
+      now apply sto_trace_app with (t1:=t1).
+    }
+    assert (tid1 > 0) as T1N. {
+      apply (trace_in_nonzero _ a1 _ TH).
+      right; now left.
+    }
+    destruct a1; destruct a2; try reflexivity.
+    all: try solve [simpl in AP; omega].
+    all: inversion TH.
+    simpl in H6; omega.
+    simpl in H5; omega.
+    simpl in H6; omega.
+  }
+
+  {
+    destruct t1; cbn in *; inversion ET; subst.
+    destruct (Nat.eq_dec tid1 tid2); [ congruence | ].
+    rewrite tid_phase_head in P; omega.
+    destruct (Nat.eq_dec tid1 tid0); [ omega | ].
+
+    constructor; auto.
+    rewrite tid_phase_swap; auto.
+    intros v I.
+    apply Permutation_in with (l:=t1 ++ (tid2, a2) :: (tid1, a1) :: t2).
+    apply Permutation_app_head; constructor.
+    apply (H0 v).
+    apply Permutation_in with (l:=t1 ++ (tid1, a1) :: (tid2, a2) :: t2).
+    apply Permutation_app_head; constructor.
+    auto.
+  }
+
+  {
+    destruct t1; cbn in *; inversion ET; subst.
+    destruct (Nat.eq_dec tid1 tid2); [ congruence | ].
+    rewrite tid_phase_head in P; omega.
+    destruct (Nat.eq_dec tid1 tid0); [ omega | ].
+
+    constructor; auto.
+    rewrite tid_phase_swap; auto.
+    rewrite locked_by_swap_head; auto.
+
+    {
+      assert (sto_trace ((tid2, a2) :: (tid1, a1) :: t2)) as TH. {
+        now apply sto_trace_app with (t1:=t1).
+      }
+      assert (tid1 > 0) as T1N. {
+        apply (trace_in_nonzero _ a1 _ TH).
+        right; now left.
+      }
+      destruct a1; destruct a2; try reflexivity.
+      all: try solve [simpl in AP; omega].
+      all: inversion TH.
+      simpl in H5; omega.
+      simpl in H4; omega.
+      simpl in H5; omega.
+    }
+
+    rewrite <- write_version_swap; auto.
+  }
+
+  {
+    destruct t1; cbn in *; inversion ET; subst.
+    destruct (Nat.eq_dec tid1 tid2); [ congruence | ].
+    rewrite tid_phase_head in P; omega.
+    destruct (Nat.eq_dec tid1 tid0); [ omega | ].
+
+    constructor; auto.
+    rewrite tid_phase_swap; auto.
+    rewrite tid_phase_swap; auto.
+  }
+
+  {
+    destruct t1; cbn in *; inversion ET.
+    rewrite <- H2 in *; rewrite H4 in *; rewrite <- H3 in *; clear H2 H3 H4.
+    destruct (Nat.eq_dec tid1 tid0); [ congruence | ].
+    rewrite tid_phase_head in P; omega.
+    destruct (Nat.eq_dec tid1 tid0); [ omega | ].
+
+    rewrite H3 in *; clear H3.
+    constructor; auto.
+    rewrite tid_phase_swap; auto.
+    rewrite locked_by_swap_head; auto.
+
+    {
+      assert (sto_trace ((tid2, a2) :: (tid1, a1) :: t2)) as TH. {
+        now apply sto_trace_app with (t1:=t1).
+      }
+      assert (tid1 > 0) as T1N. {
+        apply (trace_in_nonzero _ a1 _ TH).
+        right; now left.
+      }
+      destruct a1; destruct a2; try reflexivity.
+      all: try solve [simpl in AP; omega].
+      all: inversion TH.
+      simpl in H6; omega.
+      simpl in H5; omega.
+      simpl in H6; omega.
+    }
+  }
+
+  {
+    destruct t1; cbn in *; inversion ET.
+    {
+      subst.
+      rewrite tid_phase_head in P.
+      destruct (Nat.eq_dec tid1 tid2); [ | omega ].
+      subst; clear P; congruence.
+    }
+    rewrite <- H2 in *; clear p H2.
+    rewrite H3 in *; clear t H3 ET.
+
+    constructor; auto.
+    rewrite tid_phase_swap; auto.
+    {
+      intros vers I.
+      apply Permutation_in with (l:=t1 ++ (tid2, a2) :: (tid1, a1) :: t2).
+      apply Permutation_app_head; constructor.
+      apply (H0 vers).
+      apply Permutation_in with (l:=t1 ++ (tid1, a1) :: (tid2, a2) :: t2).
+      apply Permutation_app_head; constructor.
+      auto.
+    }
+    destruct (Nat.eq_dec tid1 tid0); auto.
+    rewrite <- e in *; clear e tid0 P.
+    admit.
+  }
+
+  {
+    destruct t1; cbn in *; inversion ET.
+    {
+      rewrite H3 in *; rewrite H5 in *; clear t tid0 H3 H5.
+      rewrite tid_phase_head in P.
+      destruct (Nat.eq_dec tid1 tid2); [ congruence | omega ].
+    }
+    rewrite <- H3 in *; rewrite H4 in *; clear p t H3 H4 ET.
+    destruct (Nat.eq_dec tid1 tid0); auto.
+    Focus 2.
+    rewrite write_version_swap; [ | omega].
+    apply complete_write_item_step with (val:=val).
+    rewrite tid_phase_swap; auto.
+    constructor.
+    eeFocus 2. auto.
+    apply IHT; auto.
+    rewrite tid_phase_swap; auto.
+    
+    rewrite locked_by_swap_head; auto.
+
+    {
+      assert (sto_trace ((tid2, a2) :: (tid1, a1) :: t2)) as TH. {
+        now apply sto_trace_app with (t1:=t1).
+      }
+      assert (tid1 > 0) as T1N. {
+        apply (trace_in_nonzero _ a1 _ TH).
+        right; now left.
+      }
+      destruct a1; destruct a2; try reflexivity.
+      all: try solve [simpl in AP; omega].
+      all: inversion TH.
+      simpl in H6; omega.
+      simpl in H5; omega.
+      simpl in H6; omega.
+    }
+    
+
+Lemma count_occ_app {A:Type} eq_dec (l1 l2:list A) x:
+  count_occ eq_dec (l1 ++ l2) x =
+  count_occ eq_dec l1 x + count_occ eq_dec l2 x.
+Proof.
+  induction l1; cbn; auto.
+  destruct (eq_dec a x); auto.
+  rewrite IHl1; omega.
+Qed.
+
+Lemma in_seq_list_subset tid t c1 c2:
+  In tid (seq_list' t c2) ->
+  (forall x, In x c2 -> In x c1) ->
+  In tid (seq_list' t c1).
+Proof.
+  revert c1 c2; induction t; intros; cbn; auto.
+  destruct a; destruct a; try solve [now apply (IHt c1 c2)].
+  cbn in H.
+  remember (count_occ Nat.eq_dec c2 t0) as c2ct; destruct c2ct.
+  destruct (count_occ Nat.eq_dec c1 t0).
+  now apply (IHt c1 c2).
+  right; now apply (IHt c1 c2).
+  assert (In t0 c1). {
+    apply H0.
+    rewrite (count_occ_In Nat.eq_dec); omega.
+  }
+  rewrite (count_occ_In Nat.eq_dec) in H1.
+  destruct (count_occ Nat.eq_dec c1 t0); try omega.
+  destruct H; [ left; auto | right; now apply (IHt c1 c2) ].
+  cbn in H.
+  assert (forall x, In x (t0 :: c2) -> In x (t0 :: c1)). {
+    intros x I; destruct I; [ left | right ]; auto.
+  }
+  now apply (IHt (t0::c1) (t0::c2)).
+Qed.
+
+Lemma count_occ_Permutation {A:Type} eq_dec (l1 l2:list A) a:
+  Permutation l1 l2 ->
+  count_occ eq_dec l1 a = count_occ eq_dec l2 a.
+Proof.
+  intros P; induction P; auto; cbn.
+  - destruct (eq_dec x a); now rewrite IHP.
+  - destruct (eq_dec x a); destruct (eq_dec y a); auto.
+  - rewrite IHP1; now rewrite IHP2.
+Qed.
+
+Lemma in_seq_list_Permutation tid t c1 c2:
+  Permutation c1 c2 ->
+  In tid (seq_list' t c1) ->
+  In tid (seq_list' t c2).
+Proof.
+  intros P I.
+  apply in_seq_list_subset with (c2:=c1); auto.
+  intros x E; apply Permutation_in with (l:=c1); auto.
+Qed.
+
+Lemma in_seq_list_or tid t x c:
+  In tid (seq_list' t (x :: c)) ->
+  tid = x \/ In tid (seq_list' t c).
+Proof.
+  revert x c; induction t; intros; cbn; auto.
+  destruct a; destruct a; try solve [now apply (IHt x c)].
+  - cbn in H.
+    destruct (Nat.eq_dec x t0).
+    + destruct H; [ subst; now left | ].
+      apply IHt in H; destruct or H; [ now left | right ].
+      destruct (count_occ Nat.eq_dec c t0); auto.
+      now right.
+    + destruct (count_occ Nat.eq_dec c t0).
+      apply IHt in H; destruct or H; auto.
+      destruct H; [ right; subst; now left | ].
+      apply IHt in H; destruct or H; [ now left | right ].
+      now right.
+  - cbn in H.
+    assert (Permutation (t0::x::c) (x::t0::c)) by (apply perm_swap).
+    apply (in_seq_list_Permutation _ _ _ _ H0) in H; clear H0.
+    apply (IHt _ _ H).
+Qed.  
+
+Lemma commit_seq_point_in_seq_list tid (t1 t2 t3:trace):
+  In tid (seq_list (t1 ++ (tid, commit_txn) :: t2 ++ (tid, seq_point) :: t3)).
+Proof.
+  induction t1.
+  cbn.
+  induction t2.
+  cbn; destruct (Nat.eq_dec tid tid).
+  cbn; now left.
+  congruence.
+  destruct a; destruct a; cbn; auto.
+  destruct (Nat.eq_dec tid t).
+  rewrite e; now left.
+  auto.
+  apply in_seq_list_subset with (c2:=[tid]); auto.
+  intros x I; destruct I; right; now left.
+
+  destruct a; destruct a; simpl; cbn; auto.
+  apply in_seq_list_subset with (c2:=[]); auto.
+  intros x I; destruct I.
+Qed.
+
+Lemma in_seq_list_iff tid t:
+  sto_trace t ->
+  tid_phase tid t = 4 <-> In tid (seq_list t).
+Proof.
+  intros T; split.
+
+  intros P.
+  apply commit_in_phase4 in P.
+  apply in_split in P.
+  destruct P as [t1 [t2 TE]].
+  assert (In (tid, seq_point) t2). {
+    apply seq_point_in_commit_in with (t1:=t1).
+    now rewrite TE in T.
+  }
+  apply in_split in H.
+  destruct H as [t2' [t3 TE']].
+  rewrite TE; rewrite TE'.
+  apply commit_seq_point_in_seq_list.
+  auto.
+
+  induction T; intros I; cbn in *; try contradiction.
+  all: try apply IHT in I.
+  all: destruct (Nat.eq_dec tid tid0); auto.
+  all: try solve [rewrite <- e in *; rewrite I in *; omega].
+  apply IHT.
+  apply in_seq_list_or in I.
+  destruct I; auto; congruence.
+Qed.
+
+Lemma serialize_not_in_head tid a t c:
+  ~ In tid c ->
+  serialize_by ((tid, a) :: t) c = serialize_by t c.
+Proof.
+  induction c; intros NI; cbn; auto.
+  destruct (Nat.eq_dec a0 tid).
+  rewrite e in NI; destruct NI; now left.
+  assert (~ In tid c) as NIX. {
+    contradict NI; now right.
+  }
+  now rewrite (IHc NIX).
+Qed.
+
+Lemma serialize_trace t:
+  sto_trace t ->
+  sto_trace (serialize t).
+Proof.
+  intros T; induction T; cbn in *; auto.
+  1-9: match goal with
+       | [ |- context [ (?tid, ?a) :: ?t ] ] =>
+         assert (tid_phase tid ((tid, a) :: t) <> 4) as NP by
+             (cbn; destruct (Nat.eq_dec tid tid); omega)
+       end.
+  1-9: rewrite in_seq_list_iff in NP; cbn in NP; auto.
+  6: now apply lock_write_item_step with (v:=v).
+  1-9: now rewrite (serialize_not_in_head _ _ _ _ NP).
+  Focus 2.
+  
+  
+
+  assert (tid_phase tid0 t
+  - cbn in *; auto.
+  - 
